src/KMS/KMSUtils.dfy
@@ -75,13 +75,144 @@ module {:extern "KMSUtils"} KMSUtils {
 
   datatype DecryptResponse = DecryptResponse(contentLength: int, httpStatusCode: HttpStatusCode, keyID: string, plaintext: seq<uint8>, responseMetadata: ResponseMetadata)
 
-  // TODO: Return Result<KMSClient>, Dafny does not currently support returning interfaces
-  trait KMSClientSupplier {
+  // TODO: Return Result<KMSClient>, Dafny does not currently support returning Result<trait>
+  trait {:termination false} KMSClientSupplier {
+    ghost var Repr: set<object>
+
+    predicate Valid()
+      reads this, Repr
+      ensures Valid() ==> this in Repr
+
     method GetClient(region: Option<string>) returns (res: Result<DefaultClient>)
   }
 
   class DefaultClientSupplier extends KMSClientSupplier {
-    constructor() {}
+    const clientSupplier: KMSClientSupplier
+
+    predicate Valid()
+      reads this, Repr
+      ensures Valid() ==> this in Repr
+    {
+      this in Repr &&
+      clientSupplier in Repr && clientSupplier.Repr <= Repr && this !in clientSupplier.Repr && clientSupplier.Valid()
+    }
+
+    constructor()
+      ensures Valid()
+    {
+      var newClientSupplier := new BaseClientSupplier();
+      this.clientSupplier := newClientSupplier;
+      Repr := {this} + newClientSupplier.Repr;
+    }
+
+    method GetClient(region: Option<string>) returns (res: Result<DefaultClient>)
+    {
+      var resClient := this.clientSupplier.GetClient(region);
+      return resClient;
+    }
+  }
+
+  // An implementation of a KMSClientSupplier that takes in an existing KMSClientSupplier as well as a seq of regions
+  // (strings). The LimitRegionsClientSupplier will only return a KMSClient from the given KMSClientSupplier if the
+  // region provided to GetClient(region) is in the list of regions associated with the LimitRegionsClientSupplier.
+  class LimitRegionsClientSupplier extends KMSClientSupplier {
+    const clientSupplier: KMSClientSupplier
+    const regions: seq<string>
+
+    predicate Valid()
+      reads this, Repr
+      ensures Valid() ==> this in Repr
+    {
+      this in Repr &&
+      clientSupplier in Repr && clientSupplier.Repr <= Repr && this !in clientSupplier.Repr && clientSupplier.Valid()
+    }
+
+    constructor(clientSupplier: KMSClientSupplier, regions: seq<string>)
+      requires clientSupplier.Valid()
+      ensures this.clientSupplier == clientSupplier
+      ensures this.regions == regions
+      ensures Valid()
+    {
+      this.clientSupplier := clientSupplier;
+      this.regions := regions;
+      Repr := {this} + clientSupplier.Repr;
+    }
+
+    method GetClient(region: Option<string>) returns (res: Result<DefaultClient>)
+      ensures region.None? ==> res.Failure?
+      ensures region.Some? && !(region.get in regions) ==> res.Failure?
+      ensures region.Some? && region.get in regions ==> res.Success?
+    {
+      // In order to limit regions, make sure our given region string exists and is a member of the regions to limit to
+      if region.Some? && region.get in regions {
+        var resClient := this.clientSupplier.GetClient(region);
+        return resClient;
+      } else {
+        return Failure("Given region not in regions maintained by LimitRegionsClientSupplier");
+      }
+    }
+  }
+
+  // An implementation of a KMSClientSupplier that takes in an existing KMSClientSupplier as well as a seq of regions
+  // (strings). The ExcludeRegionsClientSupplier will only return a KMSClient from the given KMSClientSupplier if the
+  // region provided to GetClient(region) is not in the list of regions associated with the ExcludeRegionsClientSupplier.
+  class ExcludeRegionsClientSupplier extends KMSClientSupplier {
+    const clientSupplier: KMSClientSupplier
+    const regions: seq<string>
+
+    predicate Valid()
+      reads this, Repr
+      ensures Valid() ==> this in Repr
+    {
+      this in Repr &&
+      clientSupplier in Repr && clientSupplier.Repr <= Repr && this !in clientSupplier.Repr && clientSupplier.Valid()
+    }
+
+    constructor(clientSupplier: KMSClientSupplier, regions: seq<string>)
+      requires clientSupplier.Valid()
+      ensures this.clientSupplier == clientSupplier
+      ensures this.regions == regions
+      ensures Valid()
+    {
+      this.clientSupplier := clientSupplier;
+      this.regions := regions;
+      Repr := {this} + clientSupplier.Repr;
+    }
+
+    method GetClient(region: Option<string>) returns (res: Result<DefaultClient>)
+      ensures region.None? ==> res.Success?
+      ensures region.Some? && !(region.get in regions) ==> res.Success?
+      ensures region.Some? && region.get in regions ==> res.Failure?
+    {
+      // Exclude if our regions is a member of the maintained regions
+      if region.Some? && region.get in regions {
+        return Failure("Given region is in regions maintained by ExcludeRegionsClientSupplier");
+      } else {
+        var resClient := this.clientSupplier.GetClient(region);
+        return resClient;
+      }
+    }
+  }
+
+  class BaseClientSupplier extends KMSClientSupplier {
+
+    predicate Valid()
+      reads this, Repr
+      ensures Valid() ==> this in Repr
+    {
+      this in Repr
+    }
+
+    // TODO: This needs to take in a region, and creds
+    // What we really want to do is take in a AmazonKeyManagementServiceConfig
+    // and an AWSCredentials
+    constructor()
+      ensures Valid()
+    {
+       Repr := {this};
+    }
+
+    // Since this is the base client supplier, this just calls the extern GetClient method
     method {:extern} GetClient(region: Option<string>) returns (res: Result<DefaultClient>)
   }
 
